formal/fstar/ocaml-output/HDT_Dictionary.ml
@@ -12,15 +12,16 @@ let crc8_byte (crc : Prims.nat) (b : Prims.nat) : Prims.nat=
     (crc8_step
        (crc8_step
           (crc8_step (crc8_step (crc8_step (crc8_step (crc8_step c0)))))))
-let rec crc8_range (s : Prims.string) (pos : Prims.nat) (count : Prims.nat)
-  (crc : Prims.nat) : Prims.nat FStar_Pervasives_Native.option=
+let rec crc8_range (a : HDT_Container.hdt_bytes) (pos : Prims.nat)
+  (count : Prims.nat) (crc : Prims.nat) :
+  Prims.nat FStar_Pervasives_Native.option=
   if count = Prims.int_zero
   then FStar_Pervasives_Native.Some crc
   else
-    (match HDT_Container.hex_byte s pos with
+    (match HDT_Container.byte_get a pos with
      | FStar_Pervasives_Native.None -> FStar_Pervasives_Native.None
      | FStar_Pervasives_Native.Some b ->
-         crc8_range s (pos + Prims.int_one) (count - Prims.int_one)
+         crc8_range a (pos + Prims.int_one) (count - Prims.int_one)
            (crc8_byte crc b))
 let crc32c_step (c : Prims.nat) : Prims.nat=
   if ((mod) c (Prims.of_int (2))) = Prims.int_one
@@ -35,35 +36,36 @@ let crc32c_byte (crc : Prims.nat) (b : Prims.nat) : Prims.nat=
        (crc32c_step
           (crc32c_step
              (crc32c_step (crc32c_step (crc32c_step (crc32c_step c0)))))))
-let rec crc32c_range (s : Prims.string) (pos : Prims.nat) (count : Prims.nat)
-  (crc : Prims.nat) : Prims.nat FStar_Pervasives_Native.option=
+let rec crc32c_range (a : HDT_Container.hdt_bytes) (pos : Prims.nat)
+  (count : Prims.nat) (crc : Prims.nat) :
+  Prims.nat FStar_Pervasives_Native.option=
   if count = Prims.int_zero
   then FStar_Pervasives_Native.Some crc
   else
-    (match HDT_Container.hex_byte s pos with
+    (match HDT_Container.byte_get a pos with
      | FStar_Pervasives_Native.None -> FStar_Pervasives_Native.None
      | FStar_Pervasives_Native.Some b ->
-         crc32c_range s (pos + Prims.int_one) (count - Prims.int_one)
+         crc32c_range a (pos + Prims.int_one) (count - Prims.int_one)
            (crc32c_byte crc b))
-let crc32c_of_range (s : Prims.string) (pos : Prims.nat) (count : Prims.nat)
-  : Prims.nat FStar_Pervasives_Native.option=
-  match crc32c_range s pos count (Prims.parse_int "0xFFFFFFFF") with
+let crc32c_of_range (a : HDT_Container.hdt_bytes) (pos : Prims.nat)
+  (count : Prims.nat) : Prims.nat FStar_Pervasives_Native.option=
+  match crc32c_range a pos count (Prims.parse_int "0xFFFFFFFF") with
   | FStar_Pervasives_Native.None -> FStar_Pervasives_Native.None
   | FStar_Pervasives_Native.Some c ->
       FStar_Pervasives_Native.Some
         (HDT_Container.nat_xor c (Prims.parse_int "0xFFFFFFFF")
            (Prims.of_int (32)))
-let read_u8 (s : Prims.string) (pos : Prims.nat) :
+let read_u8 (a : HDT_Container.hdt_bytes) (pos : Prims.nat) :
   Prims.nat FStar_Pervasives_Native.option=
-  match HDT_Container.hex_byte s pos with
+  match HDT_Container.byte_get a pos with
   | FStar_Pervasives_Native.None -> FStar_Pervasives_Native.None
   | FStar_Pervasives_Native.Some b -> FStar_Pervasives_Native.Some b
-let read_u32_le (s : Prims.string) (pos : Prims.nat) :
+let read_u32_le (a : HDT_Container.hdt_bytes) (pos : Prims.nat) :
   Prims.nat FStar_Pervasives_Native.option=
-  match ((HDT_Container.hex_byte s pos),
-          (HDT_Container.hex_byte s (pos + Prims.int_one)),
-          (HDT_Container.hex_byte s (pos + (Prims.of_int (2)))),
-          (HDT_Container.hex_byte s (pos + (Prims.of_int (3)))))
+  match ((HDT_Container.byte_get a pos),
+          (HDT_Container.byte_get a (pos + Prims.int_one)),
+          (HDT_Container.byte_get a (pos + (Prims.of_int (2)))),
+          (HDT_Container.byte_get a (pos + (Prims.of_int (3)))))
   with
   | (FStar_Pervasives_Native.Some b0, FStar_Pervasives_Native.Some b1,
      FStar_Pervasives_Native.Some b2, FStar_Pervasives_Native.Some b3) ->
@@ -81,19 +83,19 @@ let la_preamble_crc8_pos (la : HDT_Container.hdt_log_array_info) : Prims.nat=
   nat_sub la.HDT_Container.la_data_start Prims.int_one
 let la_crc32_pos (la : HDT_Container.hdt_log_array_info) : Prims.nat=
   nat_sub la.HDT_Container.la_end (Prims.of_int (4))
-let la_preamble_crc8_ok (s : Prims.string)
+let la_preamble_crc8_ok (a : HDT_Container.hdt_bytes)
   (la : HDT_Container.hdt_log_array_info) : Prims.bool=
-  match ((crc8_range s la.HDT_Container.la_start (la_preamble_len la)
-            Prims.int_zero), (read_u8 s (la_preamble_crc8_pos la)))
+  match ((crc8_range a la.HDT_Container.la_start (la_preamble_len la)
+            Prims.int_zero), (read_u8 a (la_preamble_crc8_pos la)))
   with
   | (FStar_Pervasives_Native.Some c, FStar_Pervasives_Native.Some stored) ->
       c = stored
   | (uu___, uu___1) -> false
-let la_data_crc32_ok (s : Prims.string)
+let la_data_crc32_ok (a : HDT_Container.hdt_bytes)
   (la : HDT_Container.hdt_log_array_info) : Prims.bool=
-  match ((crc32c_of_range s la.HDT_Container.la_data_start
+  match ((crc32c_of_range a la.HDT_Container.la_data_start
             la.HDT_Container.la_data_bytes),
-          (read_u32_le s (la_crc32_pos la)))
+          (read_u32_le a (la_crc32_pos la)))
   with
   | (FStar_Pervasives_Native.Some c, FStar_Pervasives_Native.Some stored) ->
       c = stored
@@ -104,30 +106,30 @@ let pfc_preamble_len (sec : HDT_Container.hdt_pfc_section) : Prims.nat=
        Prims.int_one) sec.HDT_Container.pfc_start
 let pfc_preamble_crc8_pos (sec : HDT_Container.hdt_pfc_section) : Prims.nat=
   nat_sub (sec.HDT_Container.pfc_blocks).HDT_Container.la_start Prims.int_one
-let pfc_preamble_crc8_ok (s : Prims.string)
+let pfc_preamble_crc8_ok (a : HDT_Container.hdt_bytes)
   (sec : HDT_Container.hdt_pfc_section) : Prims.bool=
-  match ((crc8_range s sec.HDT_Container.pfc_start (pfc_preamble_len sec)
-            Prims.int_zero), (read_u8 s (pfc_preamble_crc8_pos sec)))
+  match ((crc8_range a sec.HDT_Container.pfc_start (pfc_preamble_len sec)
+            Prims.int_zero), (read_u8 a (pfc_preamble_crc8_pos sec)))
   with
   | (FStar_Pervasives_Native.Some c, FStar_Pervasives_Native.Some stored) ->
       c = stored
   | (uu___, uu___1) -> false
-let pfc_packed_crc32_ok (s : Prims.string)
+let pfc_packed_crc32_ok (a : HDT_Container.hdt_bytes)
   (sec : HDT_Container.hdt_pfc_section) : Prims.bool=
-  match ((crc32c_of_range s sec.HDT_Container.pfc_packed_start
+  match ((crc32c_of_range a sec.HDT_Container.pfc_packed_start
             sec.HDT_Container.pfc_packed_bytes),
-          (read_u32_le s
+          (read_u32_le a
              (nat_sub sec.HDT_Container.pfc_end (Prims.of_int (4)))))
   with
   | (FStar_Pervasives_Native.Some c, FStar_Pervasives_Native.Some stored) ->
       c = stored
   | (uu___, uu___1) -> false
-let pfc_section_crc_ok (s : Prims.string)
+let pfc_section_crc_ok (a : HDT_Container.hdt_bytes)
   (sec : HDT_Container.hdt_pfc_section) : Prims.bool=
-  (((pfc_preamble_crc8_ok s sec) &&
-      (la_preamble_crc8_ok s sec.HDT_Container.pfc_blocks))
-     && (la_data_crc32_ok s sec.HDT_Container.pfc_blocks))
-    && (pfc_packed_crc32_ok s sec)
+  (((pfc_preamble_crc8_ok a sec) &&
+      (la_preamble_crc8_ok a sec.HDT_Container.pfc_blocks))
+     && (la_data_crc32_ok a sec.HDT_Container.pfc_blocks))
+    && (pfc_packed_crc32_ok a sec)
 let bit_divisor (b : Prims.nat) : Prims.pos=
   if b = Prims.int_zero
   then Prims.int_one
@@ -150,7 +152,7 @@ let bit_divisor (b : Prims.nat) : Prims.pos=
               if b = (Prims.of_int (6))
               then (Prims.of_int (64))
               else (Prims.of_int (128))
-let rec la_bits_acc (s : Prims.string) (data_start : Prims.nat)
+let rec la_bits_acc (a : HDT_Container.hdt_bytes) (data_start : Prims.nat)
   (bitpos : Prims.nat) (nbits : Prims.nat) (mult : Prims.pos)
   (acc : Prims.nat) : Prims.nat FStar_Pervasives_Native.option=
   if nbits = Prims.int_zero
@@ -158,16 +160,17 @@ let rec la_bits_acc (s : Prims.string) (data_start : Prims.nat)
   else
     (let byte_idx = data_start + (bitpos / (Prims.of_int (8))) in
      let shift = (mod) bitpos (Prims.of_int (8)) in
-     match HDT_Container.hex_byte s byte_idx with
+     match HDT_Container.byte_get a byte_idx with
      | FStar_Pervasives_Native.None -> FStar_Pervasives_Native.None
      | FStar_Pervasives_Native.Some b ->
          let bitval = (mod) (b / (bit_divisor shift)) (Prims.of_int (2)) in
-         la_bits_acc s data_start (bitpos + Prims.int_one)
+         la_bits_acc a data_start (bitpos + Prims.int_one)
            (nbits - Prims.int_one) (mult * (Prims.of_int (2)))
            (acc + (bitval * mult)))
-let la_entry (s : Prims.string) (la : HDT_Container.hdt_log_array_info)
-  (idx : Prims.nat) : Prims.nat FStar_Pervasives_Native.option=
-  la_bits_acc s la.HDT_Container.la_data_start
+let la_entry (a : HDT_Container.hdt_bytes)
+  (la : HDT_Container.hdt_log_array_info) (idx : Prims.nat) :
+  Prims.nat FStar_Pervasives_Native.option=
+  la_bits_acc a la.HDT_Container.la_data_start
     (idx * la.HDT_Container.la_numbits) la.HDT_Container.la_numbits
     Prims.int_one Prims.int_zero
 let hdt_pfc_num_blocks (sec : HDT_Container.hdt_pfc_section) : Prims.nat=
@@ -178,70 +181,70 @@ let hdt_pfc_num_blocks (sec : HDT_Container.hdt_pfc_section) : Prims.nat=
   else
     (sec.HDT_Container.pfc_blocks).HDT_Container.la_numentries -
       Prims.int_one
-let pfc_block_abs_start (s : Prims.string)
+let pfc_block_abs_start (a : HDT_Container.hdt_bytes)
   (sec : HDT_Container.hdt_pfc_section) (b : Prims.nat) :
   Prims.nat FStar_Pervasives_Native.option=
-  match la_entry s sec.HDT_Container.pfc_blocks b with
+  match la_entry a sec.HDT_Container.pfc_blocks b with
   | FStar_Pervasives_Native.None -> FStar_Pervasives_Native.None
   | FStar_Pervasives_Native.Some rel ->
       FStar_Pervasives_Native.Some (sec.HDT_Container.pfc_packed_start + rel)
-let pfc_read_first (s : Prims.string) (pos : Prims.nat) :
+let pfc_read_first (a : HDT_Container.hdt_bytes) (pos : Prims.nat) :
   (Prims.string * Prims.nat) FStar_Pervasives_Native.option=
-  match HDT_Container.scan_nul s pos (FStar_String.strlen s) with
+  match HDT_Container.scan_nul a pos (HDT_Container.byte_len a) with
   | FStar_Pervasives_Native.None -> FStar_Pervasives_Native.None
   | FStar_Pervasives_Native.Some nul_pos ->
-      (match HDT_Container.bytes_to_string s pos (nul_pos - pos) with
+      (match HDT_Container.bytes_to_string a pos (nul_pos - pos) with
        | FStar_Pervasives_Native.None -> FStar_Pervasives_Native.None
        | FStar_Pervasives_Native.Some str ->
            FStar_Pervasives_Native.Some (str, (nul_pos + Prims.int_one)))
-let pfc_read_suffix (s : Prims.string) (pos : Prims.nat)
+let pfc_read_suffix (a : HDT_Container.hdt_bytes) (pos : Prims.nat)
   (prev : Prims.string) :
   (Prims.string * Prims.nat) FStar_Pervasives_Native.option=
-  match HDT_Container.vbyte_decode s pos with
+  match HDT_Container.vbyte_decode a pos with
   | FStar_Pervasives_Native.None -> FStar_Pervasives_Native.None
   | FStar_Pervasives_Native.Some (plen, p1) ->
       if plen > (FStar_String.strlen prev)
       then FStar_Pervasives_Native.None
       else
-        (match HDT_Container.scan_nul s p1 (FStar_String.strlen s) with
+        (match HDT_Container.scan_nul a p1 (HDT_Container.byte_len a) with
          | FStar_Pervasives_Native.None -> FStar_Pervasives_Native.None
          | FStar_Pervasives_Native.Some nul_pos ->
-             (match HDT_Container.bytes_to_string s p1 (nul_pos - p1) with
+             (match HDT_Container.bytes_to_string a p1 (nul_pos - p1) with
               | FStar_Pervasives_Native.None -> FStar_Pervasives_Native.None
               | FStar_Pervasives_Native.Some suffix ->
                   let prefix = FStar_String.sub prev Prims.int_zero plen in
                   FStar_Pervasives_Native.Some
                     ((Prims.strcat prefix suffix), (nul_pos + Prims.int_one))))
-let rec pfc_walk_suffixes (s : Prims.string) (at : Prims.nat)
+let rec pfc_walk_suffixes (a : HDT_Container.hdt_bytes) (at : Prims.nat)
   (prev : Prims.string) (remaining : Prims.pos) :
   Prims.string FStar_Pervasives_Native.option=
-  match pfc_read_suffix s at prev with
+  match pfc_read_suffix a at prev with
   | FStar_Pervasives_Native.None -> FStar_Pervasives_Native.None
   | FStar_Pervasives_Native.Some (str, at') ->
       if remaining = Prims.int_one
       then FStar_Pervasives_Native.Some str
-      else pfc_walk_suffixes s at' str (remaining - Prims.int_one)
-let rec decode_block_acc (s : Prims.string) (pos : Prims.nat)
+      else pfc_walk_suffixes a at' str (remaining - Prims.int_one)
+let rec decode_block_acc (a : HDT_Container.hdt_bytes) (pos : Prims.nat)
   (prev : Prims.string) (remaining : Prims.nat)
   (acc : Prims.string Prims.list) :
   Prims.string Prims.list FStar_Pervasives_Native.option=
   if remaining = Prims.int_zero
   then FStar_Pervasives_Native.Some (FStar_List_Tot_Base.rev acc)
   else
-    (match pfc_read_suffix s pos prev with
+    (match pfc_read_suffix a pos prev with
      | FStar_Pervasives_Native.None -> FStar_Pervasives_Native.None
      | FStar_Pervasives_Native.Some (str, pos') ->
-         decode_block_acc s pos' str (remaining - Prims.int_one) (str :: acc))
-let decode_block (s : Prims.string) (block_start : Prims.nat)
+         decode_block_acc a pos' str (remaining - Prims.int_one) (str :: acc))
+let decode_block (a : HDT_Container.hdt_bytes) (block_start : Prims.nat)
   (count : Prims.nat) :
   Prims.string Prims.list FStar_Pervasives_Native.option=
   if count = Prims.int_zero
   then FStar_Pervasives_Native.None
   else
-    (match pfc_read_first s block_start with
+    (match pfc_read_first a block_start with
      | FStar_Pervasives_Native.None -> FStar_Pervasives_Native.None
      | FStar_Pervasives_Native.Some (first, pos1) ->
-         decode_block_acc s pos1 first (count - Prims.int_one) [first])
+         decode_block_acc a pos1 first (count - Prims.int_one) [first])
 let block_string_count (sec : HDT_Container.hdt_pfc_section)
   (numblocks : Prims.nat) (b : Prims.nat) : Prims.nat=
   if (b + Prims.int_one) = numblocks
@@ -249,29 +252,31 @@ let block_string_count (sec : HDT_Container.hdt_pfc_section)
     nat_sub sec.HDT_Container.pfc_numstrings
       (b * sec.HDT_Container.pfc_blocksize)
   else sec.HDT_Container.pfc_blocksize
-let rec decode_section_acc (s : Prims.string)
+let rec decode_section_acc (a : HDT_Container.hdt_bytes)
   (sec : HDT_Container.hdt_pfc_section) (block_idx : Prims.nat)
   (numblocks : Prims.nat) (acc : Prims.string Prims.list) :
   Prims.string Prims.list FStar_Pervasives_Native.option=
   if block_idx >= numblocks
   then FStar_Pervasives_Native.Some acc
   else
-    (match pfc_block_abs_start s sec block_idx with
+    (match pfc_block_abs_start a sec block_idx with
      | FStar_Pervasives_Native.None -> FStar_Pervasives_Native.None
      | FStar_Pervasives_Native.Some bstart ->
          let count = block_string_count sec numblocks block_idx in
-         (match decode_block s bstart count with
+         (match decode_block a bstart count with
           | FStar_Pervasives_Native.None -> FStar_Pervasives_Native.None
           | FStar_Pervasives_Native.Some strs ->
-              decode_section_acc s sec (block_idx + Prims.int_one) numblocks
+              decode_section_acc a sec (block_idx + Prims.int_one) numblocks
                 (FStar_List_Tot_Base.op_At acc strs)))
-let decode_section (s : Prims.string) (sec : HDT_Container.hdt_pfc_section) :
+let decode_section (a : HDT_Container.hdt_bytes)
+  (sec : HDT_Container.hdt_pfc_section) :
   Prims.string Prims.list FStar_Pervasives_Native.option=
   if sec.HDT_Container.pfc_numstrings = Prims.int_zero
   then FStar_Pervasives_Native.Some []
-  else decode_section_acc s sec Prims.int_zero (hdt_pfc_num_blocks sec) []
-let pfc_extract (s : Prims.string) (sec : HDT_Container.hdt_pfc_section)
-  (id : Prims.pos) : Prims.string FStar_Pervasives_Native.option=
+  else decode_section_acc a sec Prims.int_zero (hdt_pfc_num_blocks sec) []
+let pfc_extract (a : HDT_Container.hdt_bytes)
+  (sec : HDT_Container.hdt_pfc_section) (id : Prims.pos) :
+  Prims.string FStar_Pervasives_Native.option=
   if
     (id > sec.HDT_Container.pfc_numstrings) ||
       (sec.HDT_Container.pfc_blocksize = Prims.int_zero)
@@ -280,22 +285,22 @@ let pfc_extract (s : Prims.string) (sec : HDT_Container.hdt_pfc_section)
     (let rank = id - Prims.int_one in
      let block_idx = rank / sec.HDT_Container.pfc_blocksize in
      let offset = (mod) rank sec.HDT_Container.pfc_blocksize in
-     match pfc_block_abs_start s sec block_idx with
+     match pfc_block_abs_start a sec block_idx with
      | FStar_Pervasives_Native.None -> FStar_Pervasives_Native.None
      | FStar_Pervasives_Native.Some bstart ->
-         (match pfc_read_first s bstart with
+         (match pfc_read_first a bstart with
           | FStar_Pervasives_Native.None -> FStar_Pervasives_Native.None
           | FStar_Pervasives_Native.Some (first, pos1) ->
               if offset = Prims.int_zero
               then FStar_Pervasives_Native.Some first
-              else pfc_walk_suffixes s pos1 first offset))
-let pfc_block_first_string (s : Prims.string)
+              else pfc_walk_suffixes a pos1 first offset))
+let pfc_block_first_string (a : HDT_Container.hdt_bytes)
   (sec : HDT_Container.hdt_pfc_section) (block_idx : Prims.nat) :
   Prims.string FStar_Pervasives_Native.option=
-  match pfc_block_abs_start s sec block_idx with
+  match pfc_block_abs_start a sec block_idx with
   | FStar_Pervasives_Native.None -> FStar_Pervasives_Native.None
   | FStar_Pervasives_Native.Some bstart ->
-      (match pfc_read_first s bstart with
+      (match pfc_read_first a bstart with
        | FStar_Pervasives_Native.None -> FStar_Pervasives_Native.None
        | FStar_Pervasives_Native.Some (first, uu___) ->
            FStar_Pervasives_Native.Some first)
@@ -307,7 +312,7 @@ let rec pfc_index_of (target : Prims.string) (strs : Prims.string Prims.list)
       if x = target
       then FStar_Pervasives_Native.Some idx
       else pfc_index_of target rest (idx + Prims.int_one)
-let rec pfc_find_block (s : Prims.string)
+let rec pfc_find_block (a : HDT_Container.hdt_bytes)
   (sec : HDT_Container.hdt_pfc_section) (target : Prims.string)
   (lo : Prims.nat) (hi : Prims.nat) :
   Prims.nat FStar_Pervasives_Native.option=
@@ -315,28 +320,29 @@ let rec pfc_find_block (s : Prims.string)
   then FStar_Pervasives_Native.Some lo
   else
     (let mid = ((lo + hi) + Prims.int_one) / (Prims.of_int (2)) in
-     match pfc_block_first_string s sec mid with
+     match pfc_block_first_string a sec mid with
      | FStar_Pervasives_Native.None -> FStar_Pervasives_Native.None
      | FStar_Pervasives_Native.Some head ->
          if (head = target) || (RDF_Graph_Executable.string_lt head target)
-         then pfc_find_block s sec target mid hi
-         else pfc_find_block s sec target lo (mid - Prims.int_one))
-let pfc_locate (s : Prims.string) (sec : HDT_Container.hdt_pfc_section)
-  (target : Prims.string) : Prims.pos FStar_Pervasives_Native.option=
+         then pfc_find_block a sec target mid hi
+         else pfc_find_block a sec target lo (mid - Prims.int_one))
+let pfc_locate (a : HDT_Container.hdt_bytes)
+  (sec : HDT_Container.hdt_pfc_section) (target : Prims.string) :
+  Prims.pos FStar_Pervasives_Native.option=
   let numblocks = hdt_pfc_num_blocks sec in
   if numblocks = Prims.int_zero
   then FStar_Pervasives_Native.None
   else
-    (match pfc_find_block s sec target Prims.int_zero
+    (match pfc_find_block a sec target Prims.int_zero
              (numblocks - Prims.int_one)
      with
      | FStar_Pervasives_Native.None -> FStar_Pervasives_Native.None
      | FStar_Pervasives_Native.Some block_idx ->
          let count = block_string_count sec numblocks block_idx in
-         (match pfc_block_abs_start s sec block_idx with
+         (match pfc_block_abs_start a sec block_idx with
           | FStar_Pervasives_Native.None -> FStar_Pervasives_Native.None
           | FStar_Pervasives_Native.Some bstart ->
-              (match decode_block s bstart count with
+              (match decode_block a bstart count with
                | FStar_Pervasives_Native.None -> FStar_Pervasives_Native.None
                | FStar_Pervasives_Native.Some strs ->
                    (match pfc_index_of target strs Prims.int_zero with
@@ -346,21 +352,21 @@ let pfc_locate (s : Prims.string) (sec : HDT_Container.hdt_pfc_section)
                         FStar_Pervasives_Native.Some
                           (((block_idx * sec.HDT_Container.pfc_blocksize) + k)
                              + Prims.int_one)))))
-let hdt_term_of_string (s : Prims.string) :
+let hdt_term_of_string (dstr : Prims.string) :
   RDF_Term.rdf_term FStar_Pervasives_Native.option=
-  let len = FStar_String.strlen s in
+  let len = FStar_String.strlen dstr in
   if len = Prims.int_zero
   then FStar_Pervasives_Native.None
   else
-    (let c0 = FStar_String.index s Prims.int_zero in
+    (let c0 = FStar_String.index dstr Prims.int_zero in
      if
        (((FStar_Char.int_of_char c0) = (Prims.of_int (0x5F))) &&
           (len > Prims.int_one))
          &&
-         ((FStar_Char.int_of_char (FStar_String.index s Prims.int_one)) =
+         ((FStar_Char.int_of_char (FStar_String.index dstr Prims.int_one)) =
             (Prims.of_int (0x3A)))
      then
-       match Parser_NTriples.parse_bnode s Prims.int_zero with
+       match Parser_NTriples.parse_bnode dstr Prims.int_zero with
        | Parser_Combinators.ParseOk (b, pos) ->
            (if pos = len
             then FStar_Pervasives_Native.Some (RDF_Term.T_BNode b)
@@ -370,7 +376,7 @@ let hdt_term_of_string (s : Prims.string) :
      else
        if (FStar_Char.int_of_char c0) = (Prims.of_int (0x22))
        then
-         (match Parser_NTriples.parse_literal s Prims.int_zero with
+         (match Parser_NTriples.parse_literal dstr Prims.int_zero with
           | Parser_Combinators.ParseOk (l, pos) ->
               if pos = len
               then FStar_Pervasives_Native.Some (RDF_Term.T_Literal l)
@@ -378,8 +384,8 @@ let hdt_term_of_string (s : Prims.string) :
           | Parser_Combinators.ParseFail (uu___2, uu___3) ->
               FStar_Pervasives_Native.None)
        else
-         if RDF_Term.is_iri s
-         then FStar_Pervasives_Native.Some (RDF_Term.T_IRI s)
+         if RDF_Term.is_iri dstr
+         then FStar_Pervasives_Native.Some (RDF_Term.T_IRI dstr)
          else FStar_Pervasives_Native.None)
 let hdt_string_of_term (t : RDF_Term.rdf_term) : Prims.string=
   match t with
@@ -395,47 +401,47 @@ let uu___is_Role_Predicate (projectee : hdt_role) : Prims.bool=
   match projectee with | Role_Predicate -> true | uu___ -> false
 let uu___is_Role_Object (projectee : hdt_role) : Prims.bool=
   match projectee with | Role_Object -> true | uu___ -> false
-let hdt_id_to_term (s : Prims.string) (inv : HDT_Container.hdt_inventory)
-  (role : hdt_role) (id : Prims.pos) :
+let hdt_id_to_term (a : HDT_Container.hdt_bytes)
+  (inv : HDT_Container.hdt_inventory) (role : hdt_role) (id : Prims.pos) :
   RDF_Term.rdf_term FStar_Pervasives_Native.option=
   let nshared =
     (inv.HDT_Container.inv_dict_shared).HDT_Container.pfc_numstrings in
   let extracted =
     match role with
     | Role_Predicate ->
-        pfc_extract s inv.HDT_Container.inv_dict_predicates id
+        pfc_extract a inv.HDT_Container.inv_dict_predicates id
     | Role_Subject ->
         if id <= nshared
-        then pfc_extract s inv.HDT_Container.inv_dict_shared id
-        else pfc_extract s inv.HDT_Container.inv_dict_subjects (id - nshared)
+        then pfc_extract a inv.HDT_Container.inv_dict_shared id
+        else pfc_extract a inv.HDT_Container.inv_dict_subjects (id - nshared)
     | Role_Object ->
         if id <= nshared
-        then pfc_extract s inv.HDT_Container.inv_dict_shared id
-        else pfc_extract s inv.HDT_Container.inv_dict_objects (id - nshared) in
+        then pfc_extract a inv.HDT_Container.inv_dict_shared id
+        else pfc_extract a inv.HDT_Container.inv_dict_objects (id - nshared) in
   match extracted with
   | FStar_Pervasives_Native.None -> FStar_Pervasives_Native.None
   | FStar_Pervasives_Native.Some str -> hdt_term_of_string str
-let hdt_term_to_id (s : Prims.string) (inv : HDT_Container.hdt_inventory)
-  (role : hdt_role) (term : RDF_Term.rdf_term) :
-  Prims.pos FStar_Pervasives_Native.option=
+let hdt_term_to_id (a : HDT_Container.hdt_bytes)
+  (inv : HDT_Container.hdt_inventory) (role : hdt_role)
+  (term : RDF_Term.rdf_term) : Prims.pos FStar_Pervasives_Native.option=
   let dstr = hdt_string_of_term term in
   let nshared =
     (inv.HDT_Container.inv_dict_shared).HDT_Container.pfc_numstrings in
   match role with
-  | Role_Predicate -> pfc_locate s inv.HDT_Container.inv_dict_predicates dstr
+  | Role_Predicate -> pfc_locate a inv.HDT_Container.inv_dict_predicates dstr
   | Role_Subject ->
-      (match pfc_locate s inv.HDT_Container.inv_dict_shared dstr with
+      (match pfc_locate a inv.HDT_Container.inv_dict_shared dstr with
        | FStar_Pervasives_Native.Some id -> FStar_Pervasives_Native.Some id
        | FStar_Pervasives_Native.None ->
-           (match pfc_locate s inv.HDT_Container.inv_dict_subjects dstr with
+           (match pfc_locate a inv.HDT_Container.inv_dict_subjects dstr with
             | FStar_Pervasives_Native.None -> FStar_Pervasives_Native.None
             | FStar_Pervasives_Native.Some id ->
                 FStar_Pervasives_Native.Some (nshared + id)))
   | Role_Object ->
-      (match pfc_locate s inv.HDT_Container.inv_dict_shared dstr with
+      (match pfc_locate a inv.HDT_Container.inv_dict_shared dstr with
        | FStar_Pervasives_Native.Some id -> FStar_Pervasives_Native.Some id
        | FStar_Pervasives_Native.None ->
-           (match pfc_locate s inv.HDT_Container.inv_dict_objects dstr with
+           (match pfc_locate a inv.HDT_Container.inv_dict_objects dstr with
             | FStar_Pervasives_Native.None -> FStar_Pervasives_Native.None
             | FStar_Pervasives_Native.Some id ->
                 FStar_Pervasives_Native.Some (nshared + id)))
